adding some partial progress

intermediate/Veritas.Intermediate.Verifier.fst
@@ -17,6 +17,11 @@ type vtls =
     hevict : MH.ms_hash_value ->
     vtls
 
+let update_thread_store (vs:vtls {Valid? vs})
+                        (st:S.vstore)
+                        : vtls =
+  match vs with
+  | Valid id _ clock hadd hevict -> Valid id st clock hadd hevict
 
 let thread_store (vs:vtls { Valid? vs } )
   : S.vstore
@@ -24,12 +29,121 @@ let thread_store (vs:vtls { Valid? vs } )
 
 let vget (s:slot_id) (v:data_value) (vs: vtls {Valid? vs}): vtls =
   let st = thread_store vs in
-  (* check store contains key *)
-  if not (S.store_contains st s) then Failed
-  (* check stored value is v *)
+  (* check if store contains slot s *)
+  if not (S.contains_record st s) then Failed
+  (* check if stored value is v *)
   else let Some r = S.get_record st s in
        if not (DVal? r.record_value)
        then Failed
        else if to_data_value r.record_value <> v
        then Failed
        else vs
+
+let vput (s:slot_id) (v:data_value) (vs: vtls {Valid? vs}): vtls =
+  let st = thread_store vs in
+  (* check if store contains slot s *)
+  if not (S.contains_record st s) then Failed
+  else update_thread_store vs (S.update_record_value st s (DVal v))
+
+let vaddm (s:slot_id) (r:Veritas.Intermediate.Common.record) (s':slot_id) (vs: vtls {Valid? vs}): vtls =
+  let st = thread_store vs in
+  if s > Seq.length st then Failed
+  //let { record_key = k; record_value = v } = r in
+  else let k = r.record_key in
+  let v = r.record_value in
+  (* the store should contain slot s' *)
+  if not (S.contains_record st s') then Failed
+  else 
+    let Some r' = S.get_record st s' in
+    let { 
+          record_key = k';
+          record_value = v';
+          record_add_method = a;
+          record_l_child_in_store = l_in_store;
+          record_r_child_in_store = r_in_store
+        } = r' in 
+    (* k should be a proper desc of k' *)
+    if not (Veritas.BinTree.is_proper_desc k k') then Failed
+    (* the store should not contain slot s *)
+    else if S.contains_record st s then Failed
+    (* the type of v should be consistent with k *)
+    else if not (is_value_of k v) then Failed
+    (* v' should be a merkle value *)
+    else if DVal? v' then Failed 
+    else
+      let v' = to_merkle_value v' in
+      let d = Veritas.BinTree.desc_dir k k' in
+      let dh' = desc_hash_dir v' d in 
+      (* check whether k is already in the store *)
+      if Veritas.BinTree.Left? d && Desc? dh' && l_in_store then Failed
+      else if Veritas.BinTree.Right? d && Desc? dh' && r_in_store then Failed
+      else let h = Veritas.Hash.hashfn v in
+      match dh' with
+      | Empty -> if v = init_value k then
+                   let v'_upd = Veritas.Verifier.update_merkle_value v' d k h false in
+                   let st_upd = S.update_record_value st s' (MVal v'_upd) in
+                   let st_upd2 = S.add_record st_upd s k v Veritas.Verifier.MAdd in
+                   update_thread_store vs st_upd2
+                 else Failed
+      | Desc k2 h2 b2 -> if k2 = k then
+                           if h2 = h && b2 = false then
+                             update_thread_store vs (S.add_record st s k v Veritas.Verifier.MAdd)
+                           else Failed
+                         else if v <> init_value k then Failed
+                         else if not (Veritas.BinTree.is_proper_desc k2 k) then Failed
+                         else
+                           let d2 = Veritas.BinTree.desc_dir k2 k in
+                           let mv = to_merkle_value v in
+                           let mv_upd = Veritas.Verifier.update_merkle_value mv d2 k2 h2 b2 in
+                           let v'_upd = Veritas.Verifier.update_merkle_value v' d k h false in
+                           let st_upd = S.update_record_value st s' (MVal  v'_upd) in // need to update s' to say that the child in direction d is present
+                           let st_upd2 = S.add_record st_upd s k (MVal mv_upd) Veritas.Verifier.MAdd in
+                           update_thread_store vs st_upd2
+
+
+// vevictm
+
+// vaddb
+
+// vevictb
+
+// vevictbm
+
+
+(* Per invariant.md, we will want to prove something like the following for
+   each operation OP above.
+
+High:   hst ----------OP----------> hst'
+         ^                           ^
+         .                           .
+         .                           .
+        inv                         inv
+         .                           .
+         .                           .
+         v                           v
+Low:    lst ----------OP----------> lst'
+
+  Where hst is the high-level state (Veritas.Verifier.vtls) and lst is the
+  low-level state (Veritas.Intermediate.Verifier.vtls).
+
+  We should be able to do this by showing that, during proper execution, 
+  Veritas.Intermediate.Store behaves just like a key-value store.
+
+
+let store_is_map store =
+    //1. keys are unique
+    (forall s0 s1 in store. store[s0].record_key <> store[s1].record_key) /\
+    //2. in store bits unset means that descendent is not in store
+    (forall s in store, (d:direction).
+         let r = store[s] in
+         let dh = descendent d r in
+         not (r.in_store d) ==>
+         (forall s' in store. store[s'].record_key <> dh.key)) /\
+    //3. descendent edges are to the nearest descendent
+    (forall s in store, (d:direction).
+        let r = store [s] in
+        let dh = descendent d r in
+        (forall s' in store.
+            not (dh.key < store[s'].record_key < r.record_key))
+
+*)
