intermediate/Veritas.Intermediate.Store.fsti
@@ -3,20 +3,27 @@ open FStar.Integers
 open Veritas.Intermediate.Common
 module U16 = FStar.UInt16
 module SA = Veritas.SeqAux
+module R = Veritas.Record
 
 let vstore = Seq.seq (option record)
+let st_index (st:vstore) = SA.seq_index st
 
 let get_record (st:vstore) (s:slot_id)
   : option record
   = if s >= Seq.length st then None else Seq.index st s
 
-let store_contains (st:vstore) (s:slot_id)
+let contains_record (st:vstore) (s:slot_id)
   : bool
   = Some? (get_record st s)
 
-let update_record (st:vstore) (s:SA.seq_index st) (r:record)
+let update_record (st:vstore) (s:st_index st) (r:record)
   : vstore
   = Seq.upd st s (Some r)
+
+let update_record_value (st:vstore) (s:st_index st{contains_record st s}) (v:value)
+  : vstore
+  = let Some r = get_record st s in
+    update_record st s ({r with record_value = v}) 
 
 let add_record (st:vstore) (s:SA.seq_index st) (k:key) (v:value{Veritas.Record.is_value_of k v}) (a:add_method)
   : vstore
